Port ChangeAlphabet to new tape_contains

TM/Code/ChangeAlphabet.v
@@ -63,6 +63,13 @@ Proof.
 Qed.
 
 
+Lemma map_cons' (A B: Type) (f: A->B) (ls: list A) (y: B) (ys: list B) :
+  map f ls = y :: ys ->
+  exists x xs, ls = x :: xs /\
+          y = f x /\
+          ys = map f xs.
+Proof. induction ls; intros H; cbn in *; inv H; eauto. Qed.
+
 
 Section MapCode.
   Variable sig tau : finType.
@@ -91,106 +98,106 @@ Section MapCode.
 
 
 
-  Lemma encodeTranslate_sig (x : X) (t : tape (sig^+)) :
-    tape_encodes _ t x <-> tape_encodes _ (injectTape t) x.
+  Lemma contains_translate_sig (x : X) (t : tape (sig^+)) :
+    t ≃ x <-> (injectTape t) ≃ x.
   Proof.
-    split; intros (r1&r2&H1&H2); hnf in *; cbn in *.
-    - exists (injectSymbols f' r1), (injectSymbols f' r2). hnf. cbn. split; [ clear H2 | clear H1 ].
-      + unfold injectTape, injectSymbols. simpl_tape. rewrite H1. cbn in *. reflexivity.
-      + unfold injectTape, injectSymbols. simpl_tape. rewrite H2. cbn in *.
-        rewrite map_app, !map_map. cbn. reflexivity.
-    - exists (surjectSymbols g' (inr def) r1), (surjectSymbols g' (inr def) r2). hnf. cbn. split; [ clear H2 | clear H1 ].
-      + unfold injectTape in H1. simpl_tape in H1. 
-        replace (map f' (left t)) with (injectSymbols f' (left t)) in H1 by reflexivity.
-        pose proof (surject_inject (inr def) _ H1) as ->. cbn. reflexivity.
-      + unfold injectTape in H2. simpl_tape in H2. 
-        replace (map f' (tape_local t)) with (injectSymbols f' (tape_local t)) in H2 by reflexivity.
-        pose proof (surject_inject (inr def) _ H2) as ->.
-        cbn. f_equal. unfold surjectSymbols. rewrite !map_map. rewrite map_app. rewrite !map_map. cbn.
-        f_equal. apply map_ext. intros a. cbn. unfold surject, retract_sum_g. retract_adjoint. reflexivity.
+    split; intros (y&ys&r1&HCode&HC); subst; cbn in *; hnf.
+    - repeat eexists. cbn. rewrite HCode. cbn. eauto.
+      f_equal. rewrite !map_map. cbn. now eapply map_ext.
+    - eapply map_cons' in HCode as (y'&ys'&HCode&->&->); rename y' into y; rename ys' into ys.
+      do 2 eexists. exists (surjectSymbols g' (inr def) r1). split.
+      + rewrite HCode. eauto.
+      + enough (midtape (inl START :: surjectSymbols TRetr_g (inr def) r1) 
+                        (inr y) (map inr ys) =
+                surjectTape (midtape (inl START :: r1) (inr (f y)) (map inr (map f ys)))) as L.
+        { unfold finType_CS in *. rewrite L. rewrite <- HC. symmetry. now apply surjectTape_injectTape. }
+        { cbn. f_equal.
+          - unfold surject. cbn. retract_adjoint. reflexivity.
+          - rewrite !map_map. apply map_ext. intros. unfold surject. cbn. retract_adjoint. reflexivity.
+        }
   Qed.
 
-  Lemma encodeTranslate_tau1 (x : X) (t : tape (tau^+)) :
-    tape_encodes _ t x -> tape_encodes _ (surjectTape t) x.
+  Lemma contains_translate_tau1 (x : X) (t : tape (tau^+)) :
+    t ≃ x -> surjectTape t ≃ x.
   Proof.
-    intros (r1&r2&H1&H2); hnf in *; cbn in *.
-    - exists (surjectSymbols g' (inr def) r1), (surjectSymbols g' (inr def) r2). hnf. cbn. split; [ clear H2 | clear H1 ].
-      + unfold surjectTape. unfold LiftSigmaTau.surjectTape. simpl_tape. rewrite H1. cbn. reflexivity.
-      + unfold surjectTape. unfold LiftSigmaTau.surjectTape. simpl_tape. rewrite H2. cbn.
-        rewrite !map_map, map_app, !map_map. cbn. f_equal.
-        eapply map_ext. intros a. unfold surject, retract_sum_g. retract_adjoint. reflexivity.
+    intros (y&ys&r1&HCode&->). cbn in *.
+    eapply map_cons' in HCode as (y'&ys'&HCode&->&->); rename y' into y; rename ys' into ys.
+    cbn. hnf. repeat econstructor; cbn; eauto.
+    f_equal.
+    - unfold surject. cbn. retract_adjoint. reflexivity.
+    - rewrite !map_map. apply map_ext. intros. unfold surject. cbn. retract_adjoint. reflexivity.
   Qed.
 
   
-  Lemma encodeTranslate_tau2 (x : X) (t : tape (tau^+)) :
+  Lemma contains_translate_tau2 (x : X) (t : tape (tau^+)) :
     (~ def el encode x) \/ (forall t' : tau, exists s', g t' = Some s') ->
-    tape_encodes _ (surjectTape t) x -> tape_encodes _ t x.
+    surjectTape t ≃ x -> t ≃ x.
   Proof.
-    intros HDef (r1&r2&H1&H2). hnf.
-    unfold surjectTape, LiftSigmaTau.surjectTape in *. simpl_tape in *. cbn in *.
-    
-    exists (skipn 1 (left t)). exists (skipn (S (| (encode x) |)) (tape_local t)). hnf. cbn -[skipn]. split; [clear H2 | clear H1].
-    - apply surject_cons in H1 as (s1&s2&H1&H2&H3). cbn in *. unfold surjectSymbols in *. unfold surject in *. cbn in *.
-      unfold retract_sum_g in H2. destruct s1. rewrite H1. cbn. congruence. destruct (g e); inv H2. 
-    - apply surject_app in H2 as (str1&str2&->&L1&L2). apply surject_cons in L2 as (t'&str3&->&L3&L4).
-      rewrite map_map.
-      unfold surject, retract_sum_g in L3. destruct t'; swap 1 2. destruct (g e); inv L3. inversion L3. rewrite H0 in *. clear H0 L3.
-      f_equal; [ | f_equal].
-      + apply (inject_surject (f := f')) in L1 as ->; cbn.
-        * unfold injectSymbols. cbn. unfold retract_sum_f. rewrite map_map. reflexivity.
-        * auto_inj.
-        * intros [s' | t'] Hin; swap 1 2.
-          -- unfold surjectSymbols in L1.
-             enough (exists s' : sig, g t' = Some s') as (s'&L5).
-             {
-               exists (inr s'). cbn. rewrite L5. reflexivity.
-             }
-             assert (exists x' : sig, inr x' = inr (A := bool) ((surject g def t')) /\ x' el (encode (codeable := enc_X) x)) as (x'&LH1&LH2).
-             {
-               eapply in_map_iff. rewrite <- L1. eapply in_map_iff.
-               eexists. split; eauto. unfold surject, retract_sum_g. destruct (g t'); auto.
-             }
-             inv LH1. unfold surject in LH2.
-             destruct HDef as [HDef | HDef].
-             {
-               destruct (g t').
-               - eauto.
-               - exfalso; eauto.
-             }
-             {
-               pose proof (HDef t') as (s'&?). eauto.
-             }
-          -- cbn. eauto.
-      + enough (str3 = skipn (S (| encode x |)) (str1 ++ [ inl STOP ] ++ str3)) as L by assumption.
-        rewrite app_assoc. rewrite skipn_app. reflexivity. simpl_list. cbn. rewrite Nat.add_1_r. f_equal.
-        unfold surjectSymbols in L1. apply map_length_eq in L1. auto.
+    intros HDef. intros (y&ys&rs&HCode&H). cbn in *.
+    hnf. do 2 eexists. exists (skipn 1 (left t)). split. cbn. rewrite HCode. cbn. reflexivity.
+    unfold surjectTape, LiftSigmaTau.surjectTape in H.
+
+    destruct t; cbn -[skipn] in *; inv H.
+    f_equal.
+    - eapply map_cons' in H1 as (y'&ys'H1&->&H1'&->). cbn in *. f_equal.
+      destruct y'; cbn in *; eauto. now destruct s.
+      unfold surject in H1'. cbn in H1'. destruct (g e0) eqn:E1; inv H1'.
+    - unfold surject in H2. unfold retract_sum_g in H2. destruct e; inv H2.
+      destruct (g e) eqn:E2; inv H0.
+      eapply tretract_g_inv' in E2 as ->; eauto.
+      edestruct HDef as [HDef1|HDef2].
+      { contradict HDef1. rewrite HCode. cbn. tauto. }
+      { specialize (HDef2 e) as (s'&HDef2). congruence. }
+    - rewrite map_map. 
+      change (surjectSymbols (retract_sum_g Some g) (inr def) l0 = map inr ys) in H3.
+      eapply inject_surject in H3 as ->; eauto.
+      { unfold injectSymbols. rewrite map_map. apply map_ext. intros. cbn. reflexivity. }
+      { intros. destruct HDef as [HDef1|HDef2].
+        { (* def ∉ encode x *)
+          unfold retract_sum_g. destruct t; cbn. eauto.
+          destruct (g e0) eqn:E1; cbn; eauto. 
+          contradict HDef1. rewrite HCode. cbn. right.
+          eenough (List.In (inr def) (map inr ys)) as (?&L1&L2)%in_map_iff by now inv L1.
+          rewrite <- H3. eapply in_map_iff. unfold surject. unfold retract_sum_g. cbn.
+          exists (inr e0). rewrite E1. eauto.
+        }
+        { (* retract is full *)
+          unfold retract_sum_g. destruct t; cbn; eauto.
+          destruct (g e0) eqn:E1; eauto.
+          specialize (HDef2 e0) as (?&?). congruence.
+        }
+      }
   Qed.
 
 
-  Corollary surjectTapes_sameEnc (t1 t2 : tape (sig^+)) (x : X) :
+  Corollary contains_surjectTapes_sameEnc (t1 t2 : tape (sig^+)) (x : X) :
     (~ def el encode x) \/ (forall t' : tau, exists s', g t' = Some s') ->
     surjectTape (injectTape t1) = surjectTape (injectTape t2) ->
-    tape_encodes _ t1 x -> tape_encodes _ t2 x.
+    t1 ≃ x -> t2 ≃ x.
   Proof.
     intros HDef HEq HEnc; cbn in *.
-    eapply encodeTranslate_sig. eapply encodeTranslate_tau2; auto. rewrite <- HEq.
-    eapply encodeTranslate_tau1. eapply encodeTranslate_sig. assumption.
+    eapply contains_translate_sig. eapply contains_translate_tau2; auto. rewrite <- HEq.
+    eapply contains_translate_tau1. eapply contains_translate_sig; eauto.
   Qed.
 
-  Corollary surjectTapes_sameEnc' (t1 t2 : tape (tau^+)) (x : X) :
+  Corollary contains_surjectTapes_sameEnc' (t1 t2 : tape (tau^+)) (x : X) :
     (~ def el encode x) \/ (forall t' : tau, exists s', g t' = Some s') ->
     surjectTape t1 = surjectTape t2 ->
-    tape_encodes _ t1 x -> tape_encodes _ t2 x.
+    t1 ≃ x -> t2 ≃ x.
   Proof.
     intros HDef HEq HEnc.
-    eapply encodeTranslate_tau2; auto.
-    rewrite <- HEq. now eapply encodeTranslate_tau1 in HEnc.
+    eapply contains_translate_tau2; auto.
+    rewrite <- HEq. now eapply contains_translate_tau1 in HEnc.
   Qed.
 
 
-  Lemma surjectTapes_isLeft (t : tape (tau^+)) :
-    isLeft (surjectTape t) <-> isLeft t.
-  Proof. unfold surjectTape, LiftSigmaTau.surjectTape. auto. Qed.
+  Lemma surjectTape_isRight (t : tape (tau^+)) :
+    isRight t -> isRight (surjectTape t).
+  Proof. unfold surjectTape, LiftSigmaTau.surjectTape. apply mapTape_isRight. Qed.
+
+  Lemma surjectTape_isRight' (t : tape (tau^+)) :
+    isRight (surjectTape t) -> isRight t.
+  Proof. unfold surjectTape, LiftSigmaTau.surjectTape. apply mapTape_isRight. Qed.
 
 End MapCode.
 
@@ -198,6 +205,7 @@ End MapCode.
 Hint Unfold surjectTape surjectTapes injectTape : tape.
 
 
+(* TODO: Where to put this? *)
 Definition TRetract_Retract A B : TRetract A B -> Retract A B :=
   fun tretr => {|
       Retr_g := TRetr_g;
@@ -219,7 +227,8 @@ Section Computes_Change_Alphabet.
 
   Variable (n_tapes : nat).
   Variable (i1 i2 : Fin.t n_tapes).
-  Variable (pM : {M : mTM (sig^+) (S (S n_tapes)) & states M -> unit}).
+  Variable F : finType.
+  Variable (pM : {M : mTM (sig^+) (S (S n_tapes)) & states M -> F}).
 
   Let retr' := retr' retr. 
 
@@ -227,7 +236,7 @@ Section Computes_Change_Alphabet.
   Notation "'g''" := TRetr_g.
   
 
-  Definition ChangeAlphabet : { M : mTM (tau^+) (S (S n_tapes)) & states M -> unit } :=
+  Definition ChangeAlphabet : { M : mTM (tau^+) (S (S n_tapes)) & states M -> F } :=
     LiftSigmaTau.Lift pM retr' (inr defX ::: inr defY ::: Vector.const (inr defX) n_tapes).
 
   Definition GoodCode :=
@@ -235,10 +244,12 @@ Section Computes_Change_Alphabet.
      (forall x : X, ~ defY el encode (sigma := sig) (func x))) \/
     (forall t' : tau, exists s', g' t' = Some s').
 
+
+
   Lemma ChangeAlphabet_Computes_WRealise :
-    pM ⊫ Computes_Rel cX cY func ->
+    pM ⊫ Computes_Rel func ->
     GoodCode ->
-    ChangeAlphabet ⊫ Computes_Rel _ _ func.
+    ChangeAlphabet ⊫ Computes_Rel func.
   Proof.
     unfold GoodCode.
     intros H HDef. eapply WRealise_monotone.
@@ -246,20 +257,25 @@ Section Computes_Change_Alphabet.
       unfold ChangeAlphabet. eapply Lift_WRealise; eauto.
     }
     {
-      hnf. intros tin (()&tout) HComp.
-      cbn. intros x HEncX HIntern.
+      
+      hnf. intros tin (yout&tout) HComp.
+      cbn. intros x HEncX HOut HIntern.
       cbn in HComp. repeat autounfold with tape in HComp. simpl_vector in HComp. cbn in HComp.
 
-      unshelve eapply encodeTranslate_tau1 with (def := defX) in HEncX; eauto.
+      unshelve eapply contains_translate_tau1 with (def := defX) in HEncX; eauto.
       specialize (HComp x HEncX).
-      spec_assert HComp as (HComp1&HComp2&HComp3).
-      { intros. simpl_tape. cbn. rewrite Vector.const_nth. now eapply surjectTapes_isLeft. }
+      destruct HComp as (HComp1&HComp2&HComp3); cbn in *.
+      { now eapply surjectTape_isRight. }
+      { intros. simpl_tape. cbn. rewrite Vector.const_nth. eapply surjectTape_isRight. eauto. }
       repeat split.
-      + eapply encodeTranslate_tau2; eauto.
+      + eapply contains_translate_tau2; eauto.
         destruct HDef as [[HDef1 HDef2] | HDef1]; eauto.
-      + eapply encodeTranslate_tau2; eauto.
+      + eapply contains_translate_tau2; eauto.
         destruct HDef as [[HDef1 HDef2] | HDef1]; eauto.
-      + eauto.
+      + intros i. specialize (HComp3 i).
+        erewrite VectorSpec.nth_map2 in HComp3; eauto. cbn in HComp3. rewrite VectorSpec.const_nth in HComp3.
+        change (isRight (surjectTape defX retr tout[@Fin.FS (Fin.FS i)])) in HComp3.
+        now eapply surjectTape_isRight' in HComp3.
     }
   Qed.
   
